Add more tests

Test/dafny0/DefaultParameters.dfy
@@ -1,52 +1,190 @@
 // RUN: %dafny "%s" > "%t"
 // RUN: %diff "%s.expect" "%t"
 
-datatype List<T> = Nil | Cons(T, tail: List<T> /* := Nil*/)
+module Actuals {
+  datatype List<T> = Nil | Cons(T, tail: List<T> := Nil)
 
-method M(a: int, b: int) returns (r: int)
-  ensures r == a + 2 * b
-{
-  r := a + 2 * b;
-}
-
-function method F(a: int, b: int, c: int): int
-{
-  a + 2 * b + 3 * c
-}
-
-class Cell<U> {
-  var value: U
-  constructor (u: U)
-    ensures value == u
+  method M(a: int, b: int) returns (r: int)
+    ensures r == a + 2 * b
   {
-    value := u;
+    r := a + 2 * b;
+  }
+
+  function method F(a: int, b: int, c: int): int
+  {
+    a + 2 * b + 3 * c
+  }
+
+  class Cell<U> {
+    var value: U
+    constructor (u: U)
+      ensures value == u
+    {
+      value := u;
+    }
+  }
+
+  iterator Iter(a: int, b: int) yields (z: int) {
+  }
+
+  method ParsingActualBindings() {
+    var xs0 := Cons(5, tail := Cons(7, Nil));
+    var tuple0 := (1 := 10, 0 := 300);
+    var r0 := M(100, b := 60);
+    var x0 := F(200, c := 20, b := 10);
+    var c0 := new Cell(u := 75);
+    var iter0 := new Iter(10, b := 20);
+
+    var xs1 := Cons(5, Cons(7, Nil));
+    var tuple1 := (300, 10);
+    var r1 := M(100, 60);
+    var x1 := F(200, 10, 20);
+    var c1 := new Cell(75);
+    var iter1 := new Iter(10, 20);
+
+    assert xs0 == xs1;
+    assert tuple0 == tuple1;
+    assert r0 == r1;
+    assert x0 == x1;
+    assert c0.value == c1.value;
+    assert iter0.a == iter1.a && iter0.b == iter1.b;
   }
 }
 
-iterator Iter(a: int, b: int) yields (z: int) {
+module Termination {
+  function method R(n: nat := R(0)): nat { n } // error: failure to prove termination for R(0)
 }
 
-method ParsingActualBindings() {
-  var xs0 := Cons(5, tail := Cons(7, Nil));
-  var tuple0 := (1 := 10, 0 := 300);
-  var r0 := M(100, b := 60);
-  var x0 := F(200, c := 20, b := 10);
-  var c0 := new Cell(u := 75);
-  var iter0 := new Iter(10, b := 20);
+module TwoState {
+  class C { }
 
-  var xs1 := Cons(5, Cons(7, Nil));
-  var tuple1 := (300, 10);
-  var r1 := M(100, 60);
-  var x1 := F(200, 10, 20);
-  var c1 := new Cell(75);
-  var iter1 := new Iter(10, 20);
+  twostate predicate P0(a: C, b: C := a)
+  twostate predicate P1(a: C, new b: C := a)
+  twostate predicate P2(new a: C, b: C := a) // error: 'b' needs to have been allocated already in the old state (TODO)
+  twostate predicate P3(new a: C, new b: C := a)
+  twostate lemma L0(a: C, b: C := a)
+  twostate lemma L1(a: C, new b: C := a)
+  twostate lemma L2(new a: C, b: C := a) // error: 'b' needs to have been allocated already in the old state (TODO)
+  twostate lemma L3(new a: C, new b: C := a)
+}
 
-  assert xs0 == xs1;
-  assert tuple0 == tuple1;
-  assert r0 == r1;
-  assert x0 == x1;
-  assert c0.value == c1.value;
-  assert iter0.a == iter1.a && iter0.b == iter1.b;
+module A {
+  function method F(x: int := 5): (r: int)
+    ensures r == x
+  method M(x: int := 5) returns (r: int)
+    ensures r == x
+
+  lemma Lemma0()
+    ensures F() == 5
+  {
+  }
+}
+
+module B refines A {
+  function method F(x: int): int { x }
+  method M(x: int) returns (r: int) { r := x; }
+
+  function method F'(x: int := 6): int { x }
+  method M'(x: int := 6) returns (r: int) ensures r == x { r := x; }
+
+  lemma Lemma1()
+    ensures F() == 6
+  { // error: postcondition violation
+  }
+
+  method TestLemmas() {
+    var y := F();
+    if * {
+      Lemma0();
+      assert y == 5;
+    } else if * {
+      Lemma0();
+      assert y == 6; // error
+    } else if * {
+      Lemma1();
+      assert F() == 5 && F() == 6; // fine, since F() promises one and Lemma1() the other
+    } else if * {
+      assert F() == 5;
+      var r := M();
+      assert r == 5;
+      assert r == 7; // error
+    } else {
+      assert F'() == 6;
+      var r := M'();
+      assert r == 6;
+    }
+  }
+}
+
+module Wellformedness {
+  class C {
+    var u: int
+    const v: int
+
+    function T0(x: int := this.u): int // error: insufficient reads clause
+
+    function T1(x: int := this.v): int
+
+    function T2(c: C, x: int := c.u): int
+      reads c
+
+    function T3(c: C, x: int := c.u): int // error: insufficient reads clause (despite precondition)
+      requires c == this
+      reads this
+
+    function T4(x: int := 10, z: int := 10 / x): int // error: division by zero
+
+    function T5(x: int, z: int := 10 / x): int // error: division by zero (despite precondition)
+      requires x == 10
+
+    function T6(x: int := 3 / y, y: int := 10): int // error: division by zero (despite precondition)
+      requires y == 10
+
+    function T7(x: int := 3, y: int := 10): int
+      requires y == 8
+      requires 1 / x == 2000 // error: division by zero
+  }
+
+  method M0(x: int := 8, y: int := 10 / x) // error: division by zero
+
+  method M1(x: int, z: int := 10 / x) // error: division by zero (despite precondition)
+    requires x == 10
+
+  method M2(x: int := 3 / y, y: int := 10) // error: division by zero (despite precondition)
+    requires y == 10
+
+  method M3(x: int := 3, y: int := 10)
+    requires y == 8
+    requires 1 / x == 2000 // error: division by zero
+
+  iterator Iter0(x: int := 8, y: int := 10 / x) // error: division by zero (reported twice)
+
+  iterator Iter1(x: int, z: int := 10 / x) // error: division by zero (despite precondition) (reported twice)
+    requires x == 10
+
+  iterator Iter2(x: int := 3 / y, y: int := 10) // error: division by zero (despite precondition) (reported twice)
+    requires y == 10
+
+  iterator Iter3(x: int := 3, y: int := 10)
+    requires y == 8
+    requires 1 / x == 2000 // error: division by zero (reported twice)
+
+  datatype Dt = Dt(x: int := 8, y: int := 10 / x) // error: division by zero (reported twice)
+
+  function method Int(): int
+  function method Nat(): int
+    ensures 0 <= Nat()
+
+  function SubrangeF0(x: nat := Int()): int // error: Int() may not be a "nat"
+  method SubrangeM0(x: nat := Int()) // error: Int() may not be a "nat"
+  iterator SubrangeI0(x: nat := Int()) // error: Int() may not be a "nat"
+  datatype SubrangeD0 = D0(x: nat := Int()) // error: Int() may not be a "nat"
+
+  function SubrangeF1(x: nat := Nat()): int
+  method SubrangeM1(x: nat := Nat())
+  iterator SubrangeI1(x: nat := Nat())
+  datatype SubrangeD1 = D1(x: nat := Nat())
+
   iterator DependencyRegression(x: nat)
     // if the call graph dependencies are set up correctly, then
     requires assert 0 <= Nat(); 3 < 10  // there should be no complaints about this assertion
